wip

systems/ChordProof.v
@@ -1,6 +1,7 @@
 Require Import DynamicNet.
 Require Import Chord.
 Require Import List.
+Import ListNotations.
 Require Import Arith.
 Require Import StructTact.StructTactics.
 
@@ -19,11 +20,13 @@ Section ChordProof.
 
   Notation handle_query := (handle_query SUCC_LIST_LEN hash).
   Notation handle_query_timeout := (handle_query_timeout hash).
+  Notation send := (send addr payload).
 
   Notation global_state := (global_state addr payload data timeout).
   Notation nodes := (nodes addr payload data timeout).
   Notation failed_nodes := (failed_nodes addr payload data timeout).
   Notation sigma := (sigma addr payload data timeout).
+  Notation update := (update addr addr_eq_dec data).
 
   Notation apply_handler_result := (apply_handler_result addr addr_eq_dec payload data timeout timeout_eq_dec).
   Notation end_query := (end_query hash).
@@ -49,6 +52,19 @@ Section ChordProof.
     exists st,
       sigma gst h = Some st /\
       joined st = true /\
+      In h (nodes gst) /\
+      ~ In h (failed_nodes gst).
+
+  Definition dead_node (gst : global_state) (h : addr) : Prop :=
+    exists st,
+      sigma gst h = Some st /\
+      In h (nodes gst) /\
+      In h (failed_nodes gst).
+
+  Definition joining_node (gst : global_state) (h : addr) : Prop :=
+    exists st,
+      sigma gst h = Some st /\
+      joined st = false /\
       In h (nodes gst) /\
       ~ In h (failed_nodes gst).
 
@@ -79,10 +95,28 @@ Section ChordProof.
       | None => false
     end.
 
+  Ltac break_step :=
+    match goal with
+      | H : step_dynamic _ _ |- _ =>
+        induction H
+    end.
+
   Ltac break_live_node :=
     match goal with
       | H : live_node _ _ |- _ =>
         unfold live_node in H; break_exists; repeat break_and
+    end.
+
+  Ltac break_live_node_exists_exists :=
+    match goal with
+      | H : live_node _ _ |- _ =>
+        unfold live_node in H; break_exists_exists; repeat break_and
+    end.
+
+  Ltac break_dead_node :=
+    match goal with
+      | H : dead_node _ _ |- _ =>
+        unfold dead_node in H; break_exists; repeat break_and
     end.
 
   Theorem live_node_dec_equiv_live_node : forall gst h,
@@ -98,10 +132,11 @@ Section ChordProof.
   Qed.
 
   Definition best_succ (gst : global_state) (h s : addr) : Prop :=
-    forall st o, exists xs ys,
-      sigma gst h = Some st ->
-      map addr_of (succ_list st) = xs ++ s :: ys ->
-      (In o xs -> ~ live_node gst o) /\
+    exists st xs ys,
+      live_node gst h /\
+      sigma gst h = Some st /\
+      map addr_of (succ_list st) = xs ++ s :: ys /\
+      (forall o, In o xs -> dead_node gst o) /\
       live_node gst s.
 
   (* transitive closure of best_succ *)
@@ -115,21 +150,31 @@ Section ChordProof.
         reachable gst x to ->
         reachable gst from to.
 
+  Ltac induct_reachable :=
+    match goal with
+      | H : reachable _ _ _ |- _ =>
+        induction H
+    end.
+
   Lemma ReachableTransR : forall gst from x to,
       reachable gst from x ->
       best_succ gst x to ->
       reachable gst from to.
   Proof.
     intuition.
-    match goal with
-      | H : reachable _ _ _ |- _ => induction H
-    end.
+    induct_reachable.
     - eapply ReachableTransL.
       eauto.
       eapply ReachableSucc.
       eauto.
     - eauto using ReachableTransL.
   Qed.
+
+  Lemma ReachableTrans : forall gst from x to,
+      reachable gst from x ->
+      reachable gst x to ->
+      reachable gst from to.
+  Admitted.
 
   Definition best_succ_of (gst : global_state) (h : addr) : option addr :=
     match (sigma gst) h with
@@ -183,7 +228,13 @@ Section ChordProof.
     connected_appendages gst /\
     base_not_skipped gst.
 
-  Lemma live_node_specificity : forall gst gst' ,
+  Ltac break_invariant :=
+    match goal with
+      | H : inductive_invariant _ |- _ =>
+        unfold inductive_invariant in H; break_and
+    end.
+
+  Lemma live_node_specificity : forall gst gst',
       nodes gst = nodes gst' ->
       failed_nodes gst = failed_nodes gst' ->
       sigma gst = sigma gst' ->
@@ -448,6 +499,27 @@ Section ChordProof.
       eauto using joined_preserved_by_tick_handler, joined_preserved_by_handle_query_timeout.
   Qed.
 
+  Lemma update_fixes_other_arguments : forall f x d y,
+      y <> x ->
+      update f x d y = f y.
+  Proof.
+    unfold update.
+    intuition.
+    break_if; congruence.
+  Qed.
+
+  Lemma update_preserving_states : forall gst gst' h st st' o,
+    sigma gst h = Some st ->
+    sigma gst' = update (sigma gst) o st' ->
+    h <> o ->
+    sigma gst' h = Some st.
+  Proof.
+    intuition.
+    find_reverse_rewrite.
+    find_rewrite.
+    apply update_fixes_other_arguments; auto.
+  Qed.
+
   Lemma apply_handler_result_updates_sigma : forall h st ms nts cts e gst gst',
       gst' = apply_handler_result h (st, ms, nts, cts) e gst ->
       sigma gst' h = Some st.
@@ -492,6 +564,168 @@ Section ChordProof.
       repeat find_rewrite.
       find_injection.
       eauto.
+  Qed.
+
+  Lemma adding_nodes_does_not_affect_live_node : forall gst gst' h n st,
+      ~ In n (nodes gst) ->
+      sigma gst' = update (sigma gst) n st ->
+      nodes gst' = n :: nodes gst ->
+      failed_nodes gst' = failed_nodes gst ->
+      live_node gst h ->
+      live_node gst' h.
+  Proof.
+    intuition.
+    unfold live_node.
+    break_live_node_exists_exists.
+    repeat split.
+    * eapply update_preserving_states; eauto.
+      congruence.
+    * auto.
+    * find_rewrite.
+      eauto using in_cons.
+    * find_rewrite.
+      auto.
+  Qed.
+
+  (* reverse of the above, with additional hypothesis that h <> n. *)
+  Lemma adding_nodes_did_not_affect_live_node : forall gst gst' h n st,
+      ~ In n (nodes gst) ->
+      sigma gst' = update (sigma gst) n st ->
+      nodes gst' = n :: nodes gst ->
+      failed_nodes gst' = failed_nodes gst ->
+      live_node gst' h ->
+      h <> n ->
+      live_node gst h.
+  Proof.
+    intuition.
+    unfold live_node.
+    break_live_node_exists_exists.
+    repeat split.
+    * repeat find_reverse_rewrite.
+      find_rewrite.
+      find_rewrite.
+      find_rewrite.
+      find_rewrite.
+      symmetry.
+      apply update_fixes_other_arguments.
+      congruence.
+    * auto.
+    * repeat find_rewrite.
+      find_apply_lem_hyp in_inv.
+      break_or_hyp; congruence.
+    * find_rewrite; auto.
+  Qed.
+
+  Lemma adding_nodes_does_not_affect_dead_node : forall gst gst' h n st,
+      ~ In n (nodes gst) ->
+      sigma gst' = update (sigma gst) n st ->
+      nodes gst' = n :: nodes gst ->
+      failed_nodes gst' = failed_nodes gst ->
+      dead_node gst h ->
+      dead_node gst' h.
+  Proof.
+    intuition.
+    break_dead_node.
+    unfold dead_node.
+    eexists.
+    repeat split.
+    - eapply update_preserving_states; eauto.
+      congruence.
+    - find_rewrite.
+      eauto using in_cons.
+    - find_rewrite; auto.
+  Qed.
+
+  Lemma adding_nodes_does_not_affect_best_succ : forall gst gst' h s n st,
+      best_succ gst h s ->
+      ~ In n (nodes gst) ->
+      sigma gst' = update (sigma gst) n st ->
+      nodes gst' = n :: nodes gst ->
+      failed_nodes gst' = failed_nodes gst ->
+      best_succ gst' h s.
+  Proof.
+    unfold best_succ.
+    intuition.
+    break_exists_exists.
+    repeat split; break_and.
+    - eauto using adding_nodes_does_not_affect_live_node.
+    - eapply update_preserving_states; eauto.
+      repeat break_live_node.
+      congruence.
+    - auto.
+    - intuition.
+      find_copy_apply_hyp_hyp.
+      break_dead_node.
+      eapply adding_nodes_does_not_affect_dead_node; eauto.
+    - eauto using adding_nodes_does_not_affect_live_node.
+  Qed.
+
+  Theorem start_step_keeps_at_least_one_ring : forall h gst gst' st known k,
+        at_least_one_ring gst ->
+        can_be_node h ->
+        ~ In h (nodes gst) ->
+        (In k known -> In k (nodes gst)) ->
+        (In k known -> ~ In k (failed_nodes gst)) ->
+        (known = [] -> nodes gst = []) ->
+        nodes gst' = h :: nodes gst ->
+        failed_nodes gst' = failed_nodes gst ->
+        sigma gst' = update (sigma gst) h st ->
+        at_least_one_ring gst'.
+  Admitted.
+
+  Theorem invariant_steps_to_at_least_one_ring : forall gst gst',
+      inductive_invariant gst ->
+      step_dynamic gst gst' ->
+      at_least_one_ring gst'.
+  Proof.
+    intuition.
+    break_invariant.
+    break_step.
+    - eapply start_step_keeps_at_least_one_ring; simpl; eauto.
+    - admit.
+    - admit.
+    - admit.
+    - admit.
+    - admit.
+  Admitted.
+
+  Theorem invariant_steps_to_at_most_one_ring : forall gst gst',
+      inductive_invariant gst ->
+      step_dynamic gst gst' ->
+      at_most_one_ring gst'.
+  Admitted.
+
+  Theorem invariant_steps_to_ordered_ring : forall gst gst',
+      inductive_invariant gst ->
+      step_dynamic gst gst' ->
+      ordered_ring gst'.
+  Admitted.
+
+  Theorem invariant_steps_to_connected_appendages : forall gst gst',
+      inductive_invariant gst ->
+      step_dynamic gst gst' ->
+      connected_appendages gst'.
+  Admitted.
+
+  Theorem invariant_steps_to_base_not_skipped : forall gst gst',
+      inductive_invariant gst ->
+      step_dynamic gst gst' ->
+      base_not_skipped gst'.
+  Admitted.
+
+  Theorem invariant_is_invariant : forall gst gst',
+      inductive_invariant gst ->
+      step_dynamic gst gst' ->
+      inductive_invariant gst'.
+  Proof.
+    intuition.
+    unfold inductive_invariant.
+    repeat split.
+    - eauto using invariant_steps_to_at_least_one_ring.
+    - eauto using invariant_steps_to_at_most_one_ring.
+    - eauto using invariant_steps_to_ordered_ring.
+    - eauto using invariant_steps_to_connected_appendages.
+    - eauto using invariant_steps_to_base_not_skipped.
   Qed.
 
 End ChordProof.
